driver/PrintState.ml
@@ -1,0 +1,19 @@
+open Format
+open Camlcoq
+open Csem
+
+module Init = Initializers.Initializers (NullTag) (NullPolicy)
+module Cexec = Init.Cexec
+module Csem = Cexec.Cstrategy.Ctyping.Csem
+module Csyntax = Csem.Csyntax
+module Determinism = Csyntax.Cop.Deterministic
+module Events = Determinism.Behaviors.Smallstep.Events
+module Genv = Events.Genv
+module Mem = Genv.Mem
+
+let print_mem m =
+  Printf.printf "| ";
+  for i = 1 to 16 do
+    Printf.printf "%ld |" (ZMap.get i (PMap.get dummy (mem_contents m)))
+  done;
+  Printf.printf "\n"
