common/Tags.v
@@ -4,17 +4,41 @@ Require Import Integers.
 Require Import Floats.
 Require Import Values.
 
-Module Type Tag.
+Require Import List. Import ListNotations.
 
-(** For now we will just stick the tag type in a parameter here. *)
+Module Type Policy.
+
   Parameter tag : Type.
   Parameter tag_eq_dec : forall (t1 t2:tag), {t1 = t2} + {t1 <> t2}.
   Parameter def_tag : tag.
 
-End Tag.
+  Parameter InitPCT : tag.
 
-Module TagLib (T:Tag).
-  Export T.
+  Parameter GlobalT : ident -> tag.
+  
+  Parameter VarT : tag -> tag -> option tag.
+
+  Parameter LocalT : nat -> tag -> option (tag * tag * list tag).
+  
+  Parameter ConstT : tag.
+
+  Parameter UnopT : tag -> tag -> option (tag * tag).
+
+  Parameter BinopT : tag -> tag -> tag -> option (tag * tag).
+  
+  Parameter LoadT : tag -> tag -> tag -> list tag -> option tag.
+
+  Parameter StoreT : tag -> tag -> tag -> tag -> list tag -> option (tag * tag * list tag).
+
+  Parameter IfSplitT : tag -> tag -> option (tag * tag).
+
+  Parameter IfJoinT : tag -> tag -> option tag.
+    
+  Parameter DummyT : list tag -> option (list tag).
+End Policy.
+
+Module TagLib (P:Policy).
+  Export P.
 
   Definition atom : Type := val * tag.
   Definition atom_map (f:val -> val) (a:atom) :=
@@ -41,3 +65,98 @@ Module TagLib (T:Tag).
     apply Ptrofs.eq_dec.
   Qed.  
 End TagLib.
+
+Module NullPolicy <: Policy.
+
+  Definition tag := unit.
+  Theorem tag_eq_dec : forall (t1 t2:tag), {t1 = t2} + {t1 <> t2}.
+  Proof.
+    unfold tag. intros. left. destruct t1. destruct t2. auto.
+  Qed.
+  Definition def_tag := tt.
+  
+  Definition InitPCT : tag := tt.
+
+  Definition GlobalT (id : ident) := tt.
+  
+  Definition VarT (pct pt : tag) := Some tt.
+
+  Definition LocalT (align : nat) (pct : tag) : option (tag * tag * list tag) := Some (tt, tt, [tt]).
+  
+  Definition ConstT : tag := tt.
+  
+  Definition UnopT (pct vt : tag) : option (tag * tag) := Some (tt, tt).
+
+  Definition BinopT (pct vt1 vt2 : tag) : option (tag * tag) := Some (tt, tt).
+  
+  Definition LoadT (pct pt vt : tag) (lts : list tag) : option tag := Some tt.
+
+  Definition StoreT (pct pt ovt vt : tag) (lts : list tag) : option (tag * tag * list tag) := Some (tt, tt, [tt]).
+
+  Definition IfSplitT (pct vt : tag) : option (tag * tag) := Some (tt, tt).
+
+  Definition IfJoinT (pct opct : tag) : option tag := Some tt.
+    
+  Definition DummyT (ts : list tag) : option (list tag) := Some ts.
+
+End NullPolicy.  
+
+Module PVI <: Policy.
+  
+  Inductive myTag :=
+  | Glob (id:ident)
+  | Dyn (c:nat)
+  | X
+  .
+
+  Definition tag := myTag.
+
+  Theorem tag_eq_dec : forall (t1 t2:tag), {t1 = t2} + {t1 <> t2}.
+  Proof.
+    unfold tag. intros. repeat decide equality.
+  Qed.
+  Definition def_tag := X.
+
+  Definition InitPCT := Dyn 0.
+
+  Definition GlobalT (id : ident) := Glob id.
+  
+  Definition LocalT (align : nat) (pct : tag) : option (tag * tag * list tag) :=
+    match pct with
+    | Dyn c =>
+        Some (Dyn (S c), Dyn c, repeat (Dyn c) align)
+    | _ =>
+        None
+    end.
+
+  Definition VarT (pct pt : tag) : option tag := Some pt.
+
+  Definition ConstT : tag := X.
+  
+  Definition UnopT (pct vt : tag) : option (tag * tag) := Some (pct, vt).
+
+  Definition BinopT (pct vt1 vt2 : tag) : option (tag * tag) :=
+    match vt1, vt2 with
+    | Dyn n, X =>  Some (pct, vt1)
+    | Glob id, X => Some (pct, vt1)
+    | _, _ => Some (pct, vt2)
+    end.
+
+  Definition LoadT (pct pt vt: tag) (lts : list tag) : option tag :=
+    match pt with
+    | X => None
+    | _ => if forallb (tag_eq_dec pt) lts then Some vt else None
+    end.
+
+  Definition StoreT (pct pt ovt vt : tag) (lts : list tag) : option (tag * tag * list tag) :=
+    match pt with
+    | X => None
+    | _ => if forallb (tag_eq_dec pt) lts then Some (pct,vt,lts) else None
+    end.
+
+  Definition IfSplitT (pct vt : tag) : option (tag * tag) := Some (pct, pct).
+
+  Definition IfJoinT (pct opct : tag) : option tag := Some pct.
+    
+  Definition DummyT (ts : list tag) : option (list tag) := Some ts.
+End PVI.
