common/Memdata.v
@@ -293,8 +293,8 @@ Proof.
   intros. unfold encode_int. decEq. apply bytes_of_int_mod. auto.
 Qed.
 
-Module Memdata (T: Tag).
-  Module TLib := TagLib T.
+Module Memdata (P: Policy).
+  Module TLib := TagLib P.
   Import TLib.
 
 (** * Memory values *)
